\section{Límites Radicales}
\subsection{Resolver:}
\[ L=\lim_{x \to 1} \frac{\sqrt{2x-1}-\sqrt[3]{x}}{\sqrt{5x-1}-2}\]
Solución:
\[L=\lim_{x \to 1} \frac{(\sqrt{2x-1}-1-\sqrt[3]{x}+1)(\sqrt{5x-1}+2)}{(\sqrt{5x-1}-2)(\sqrt{5x-1}+2)}\]
\[L=\lim_{x \to 1} \frac{(\sqrt{5x-1}+2) \left(\frac{(\sqrt{2x-1}-1)(\sqrt{2x-1}+1)}{\sqrt{2x-1}+1}-\frac{(\sqrt[3]{x}-1)(\sqrt[3]{x^2}+\sqrt[3]{x}+1)}{\sqrt[3]{x^2}+\sqrt[3]{x}+1}\right)}{\sqrt{5x-1}^2-2^2}\]
\[L=\lim_{x \to 1} \frac{(\sqrt{5x-1}+2)\left(\frac{(\sqrt{(2x-1)^2}-1^2)}{\sqrt{2x-1}+1}-\frac{\sqrt[3]{x^3}-1^3}{\sqrt[3]{x^2}+\sqrt[3]{x}+1}\right)}{5x-1-4}\]
\[L=\lim_{x \to 1} \frac{(\sqrt{5x-1}+2)\left(\frac{(2x-1-1)}{\sqrt{2x-1}+1}-\frac{x-1}{\sqrt[3]{x^2}+\sqrt[3]{x}+1}\right)}{5(x-1)}\]
\[L=\lim_{x \to 1} \frac{(\sqrt{5x-1}+2)\left(\frac{2(x-1)}{\sqrt{2x-1}+1}-\frac{x-1}{\sqrt[3]{x^2}+\sqrt[3]{x}+1}\right)}{5(x-1)}\]
Factorizando la indeterminación y simplificando:
\[L=\lim_{x \to 1} \frac{(\sqrt{5x-1}+2) \cancel{(x-1)}\left(\frac{2}{\sqrt{2x-1}+1}-\frac{1}{\sqrt[3]{x^2}+\sqrt[3]{x}+1}\right)}{5\cancel{(x-1)}}\]
Evaluando:
\[L=\frac{(\sqrt{5(1)-1}+2) \left(\frac{2}{\sqrt{2(1)-1}+1}-\frac{1}{\sqrt[3]{(1)^2}+\sqrt[3]{(1)}+1}\right)}{5}\]
\[L=\frac{4\cdot \left(\frac{2}{2}-\frac{1}{3} \right)}{5}\]
\[\therefore L=\frac{8}{15}\]